Prove typing properties with casts

Declarative/Transitivity.v
@@ -28,43 +28,51 @@ Inductive sized_usub : context -> expr -> expr -> expr -> nat -> Prop :=    (* d
      G ⊢ e_int <: e_int : * | 0
  | ss_abs : forall (L:vars) (G:context) (A e1 e2 B:expr) (k1 k2:kind) n1 n2 n3,
      G ⊢ A <: A : e_kind k1 | n1 ->
-     (forall x , x \notin L -> G , x : A ⊢ B <^> x <: B <^> x : e_kind k2 | n2) ->
-     (forall x , x \notin L -> G , x : A ⊢ e1 <^> x <: e2 <^> x : B <^> x | n3) ->
+     (forall x , x \notin L -> G , x : A ⊢ B ^` x <: B ^` x : e_kind k2 | n2) ->
+     (forall x , x \notin L -> G , x : A ⊢ e1 ^` x <: e2 ^` x : B ^` x | n3) ->
      G ⊢ e_abs A e1 <: e_abs A e2 : e_pi A B | S (n1 + n2 + n3)
- | ss_pi : forall (L:vars) (G:context) (A1 B1 A2 B2:expr) (k2 k1:kind) n1 n2 n3 n4 n5,
-      G ⊢ A1 <: A1 : e_kind k1 | n1 ->
-      G ⊢ A2 <: A2 : e_kind k1 | n2 ->
-      G ⊢ A2 <: A1 : e_kind k1 | n3 ->
-      (forall x, x \notin  L -> G , x : A1 ⊢ B1 <^> x <: B1 <^> x : e_kind k2 | n4)  ->
-      (forall x, x \notin  L -> G , x : A2 ⊢ B1 <^> x <: B2 <^> x : e_kind k2 | n5)  ->
-      G ⊢ e_pi A1 B1 <: e_pi A2 B2 : e_kind k2 | S (n1 + n2 + n3 + n4 + n5)
+ | ss_pi : forall (L:vars) (G:context) (A1 B1 A2 B2:expr) (k2 k1:kind) n1 n2 n3,
+      G ⊢ A2 <: A1 : e_kind k1 | n1 ->
+      (forall x, x \notin  L -> G , x : A1 ⊢ B1 ^` x <: B1 ^` x : e_kind k2 | n2)  ->
+      (forall x, x \notin  L -> G , x : A2 ⊢ B1 ^` x <: B2 ^` x : e_kind k2 | n3)  ->
+      G ⊢ e_pi A1 B1 <: e_pi A2 B2 : e_kind k2 | S (n1 + n2 + n3)
  | ss_app : forall (G:context) (e1 e e2 B A:expr) n1 n2,
      G ⊢ e  <: e  : A        | n1 ->
      G ⊢ e1 <: e2 : e_pi A B | n2 ->
      mono_type e ->
-     G ⊢ e_app e1 e <: e_app e2 e : B <^^> e | S (n1 + n2)
+     G ⊢ e_app e1 e <: e_app e2 e : B ^^ e | S (n1 + n2)
  | ss_bind : forall (L:vars) (G:context) (A e1 e2 B:expr) (k:kind) n1 n2 n3,
      G ⊢ A <: A : e_kind k | n1 ->
-     (forall x , x \notin L -> G , x : A ⊢ B  <^> x <: B  <^> x : * | n2) ->
-     (forall x , x \notin L -> G , x : A ⊢ e1 <^> x <: e2 <^> x : B <^> x | n3) ->
-     (forall x , x \notin L -> x `notin` fv_eexpr (extract (e1 <^> x))) ->
-     (forall x , x \notin L -> x `notin` fv_eexpr (extract (e2 <^> x))) ->
+     (forall x , x \notin L -> G , x : A ⊢ B  ^` x <: B  ^` x : * | n2) ->
+     (forall x , x \notin L -> G , x : A ⊢ e1 ^` x <: e2 ^` x : B ^` x | n3) ->
+     (forall x , x \notin L -> x `notin` fv_eexpr (extract (e1 ^` x))) ->
+     (forall x , x \notin L -> x `notin` fv_eexpr (extract (e2 ^` x))) ->
      G ⊢ e_bind A e1 <: e_bind A e2 : e_all A B | S (n1 + n2 + n3)
+ | ss_castup : forall (G:context) (A e1 e2:expr) (k:kind) (B:expr) n1 n2,
+     G ⊢ A <: A : e_kind k | n1 ->
+     A ⟶ B ->
+     G ⊢ e1 <: e2 : B | n2 ->
+     G ⊢ e_castup A e1 <: e_castup A e2 : A | S (n1 + n2)
+ | ss_castdn : forall (G:context) (B e1 e2:expr) (k:kind) (A:expr) n1 n2,
+     G ⊢ B <: B : e_kind k | n1 ->
+     A ⟶ B ->
+     G ⊢ e1 <: e2 : A | n2 ->
+     G ⊢ e_castdn B e1 <: e_castdn B e2 : B | S (n1 + n2)
  | ss_forall_l : forall (L:vars) (G:context) (A B C e:expr) (k:kind) n1 n2 n3 n4,
      mono_type e ->
      G ⊢ A <: A : e_kind k | n1 ->
      G ⊢ e <: e : A        | n2 ->
-     G ⊢ B <^^> e <: C : * | n3 ->
-     (forall x, x \notin L -> G , x : A ⊢ B <^> x <: B <^> x : * | n4)  ->
+     G ⊢ B ^^ e <: C : * | n3 ->
+     (forall x, x \notin L -> G , x : A ⊢ B ^` x <: B ^` x : * | n4)  ->
      G ⊢ e_all A B <: C : * | S (n1 + n2 + n3 + n4)
  | ss_forall_r : forall (L:vars) (G:context) (A B C:expr) (k:kind) n1 n2 n3,
      G ⊢ B <: B : e_kind k | n1 ->
      G ⊢ A <: A : * | n2 ->
-     (forall x, x \notin L -> G , x : B ⊢ A <: C <^> x : * | n3) ->
+     (forall x, x \notin L -> G , x : B ⊢ A <: C ^` x : * | n3) ->
      G ⊢ A <: e_all B C : * | S (n1 + n2 + n3)
  | ss_forall : forall (L:vars) (G:context) (A B C:expr) (k:kind) n1 n2,
      G ⊢ A <: A : e_kind k | n1 ->
-     (forall x, x \notin L -> G , x : A ⊢ B <^> x <: C <^> x : * | n2)  ->
+     (forall x, x \notin L -> G , x : A ⊢ B ^` x <: C ^` x : * | n2)  ->
      G ⊢ e_all A B <: e_all A C : * | S (n1 + n2)
  | ss_sub : forall (G:context) (e1 e2 B A:expr) (k:kind) n1 n2,
      G ⊢ e1 <: e2 : A | n1 ->
@@ -119,6 +127,8 @@ Proof.
   - pick fresh x and apply ss_bind; eauto.
     solve_weakening_with H0.
     solve_weakening_with H2.
+  - eauto.
+  - eauto.
   - pick fresh x and apply ss_forall_l; eauto.
     solve_weakening_with H1.
   - pick fresh x and apply ss_forall_r; eauto.
@@ -141,7 +151,7 @@ Qed.
 
 Ltac find_open_inequality_impl e :=
   match e with
-  | context [([_ / ?x] _) <^> ?x'] => assert (x' <> x) by auto 2
+  | context [([_ / ?x] _) ^` ?x'] => assert (x' <> x) by auto 2
   end
 .
 
@@ -235,7 +245,7 @@ Proof.
   - pick_fresh_with_dom_and_apply ss_pi; eauto.
     + assoc_goal_and_apply H0. eapply wf_cons; eauto.
     + assoc_goal_and_apply H2. eapply wf_cons; eauto.
-  - rewrite subst_open_distr; eauto using subst_mono.
+  - rewrite subst_open_distr; eauto.
   - pick_fresh_with_dom_and_apply ss_bind; eauto.
     + assoc_goal_and_apply H0. eapply wf_cons; eauto.
     + assoc_goal_and_apply H2. eapply wf_cons; eauto.
@@ -243,9 +253,10 @@ Proof.
       eauto 4 using fv_subst_inclusion.
     + rewrite subst_open_var_assoc, subst_extract; auto 2.
       eauto 4 using fv_subst_inclusion.
+  - eauto using reduce_subst.
+  - eauto using reduce_subst.
   - apply ss_forall_l with
       (add x (add x' L) `union` dom (Γ1 , x' : A ,, [`x' // x] Γ2)) ([`x' / x] e) k; eauto.
-    + apply subst_mono; auto.
     + rewrite <- subst_open_distr; eauto.
     + intros. assoc_goal_and_apply H1. eapply wf_cons; eauto.
   - pick_fresh_with_dom_and_apply ss_forall_r; eauto.
@@ -274,31 +285,20 @@ Ltac reconstruct_sub :=
       let H := fresh "Sub" in assert (H : Γ ⊢ e1 <: e2 : A) by eauto 3
   end.
 
-Ltac instantiate_LN_IH x :=
-  repeat
-    match goal with
-    | H : forall (x : atom), x `notin` ?L -> exists n, _ |- _ =>
-      let Fr := fresh "Fr" in
-      let IH := fresh "IH" in
-      assert (Fr : x `notin` L) by auto;
-      specialize (H x Fr); clear Fr;
-      rename H into IH
-    | H : forall (x : atom), x `notin` ?L -> _ ⊢ _ <: _ : _ |- _ =>
-       let Fr := fresh "Fr" in
-       assert (Fr : x `notin` L) by auto;
-       specialize (H x Fr); clear Fr
-    end; destruct_exists
-.
-
 Ltac discover_fresh_dom x :=
   match goal with
   | H : ?Γ, x : ?A ⊢ _ <: _ : _ |- _ =>
     let Fr := fresh "Fr" in
-    assert (Fr : x `notin` dom Γ) by
-      (let H := fresh "H" in
-       assert (H : ⊢ Γ, x : A) by auto; inversion H; now subst)
+    assert (Fr : x `notin` dom Γ) by eauto with wf sized
   end
 .
+
+Lemma wf_cons_notin_dom : forall Γ x A,
+    ⊢ Γ, x : A -> x `notin` dom Γ.
+Proof. intros. now inversion H. Qed.
+
+Hint Resolve wf_cons_notin_dom : sized.
+
 
 Ltac conclude_freshness_of x e :=
   match goal with
@@ -321,16 +321,16 @@ Ltac discover_fresh_expr x :=
     end; simpl in *; clear_dups
 .
 
-
-Ltac instantiate_LN_IH_with_fresh :=
-  let x := fresh "x" in
-  pick fresh x; instantiate_LN_IH x;
-  discover_fresh_dom x; discover_fresh_expr x
+Ltac conclude_freshes :=
+  match goal with
+  | _ : ?x `notin` ?L |- _ =>
+    discover_fresh_dom x; discover_fresh_expr x
+  end
 .
 
 Ltac rewrite_open_or_subst e x x0 :=
   match e with
-  | ?e' <^> x0 => rewrite (open_subst_eq e' x); eauto
+  | ?e' ^` x0 => rewrite (open_subst_eq e' x); eauto
   | _ => replace e with ([`x0 / x] e) by
     solve [reflexivity | rewrite fresh_subst_eq; auto ]
   end
@@ -338,15 +338,16 @@ Ltac rewrite_open_or_subst e x x0 :=
 
 Ltac rewrite_for_rename :=
   match goal with
-  | _ : ?x `notin` dom ?Γ |- _ =>
-    match goal with
-    | |- Γ, ?x0 : _ ⊢ ?e1 <: ?e1 : ?e2 | _ =>
+  | _ : ?x `notin` dom ?Γ |- ?Γ, ?x0 : _ ⊢ ?e1 <: ?e2 : ?e3 | _ =>
+    match x with
+    | x0 => fail 1
+    | _ =>
+      rewrite_open_or_subst e3 x x0;
       rewrite_open_or_subst e1 x x0;
-      rewrite_open_or_subst e2 x x0
-    | |- Γ, ?x0 : _ ⊢ ?e1 <: ?e2 : ?e3 | _ =>
-      rewrite_open_or_subst e1 x x0;
-      rewrite_open_or_subst e2 x x0;
-      rewrite_open_or_subst e3 x x0
+      match e1 with
+      | e2 => idtac
+      | _ => rewrite_open_or_subst e2 x x0
+      end
     end
   end
 .
@@ -355,24 +356,58 @@ Ltac solve_unsized_sized_with H :=
   pick_fresh_with_dom_and_apply H; eauto;
   rewrite_for_rename; apply sized_renaming_cons; eauto.
 
+Set Ltac Backtrace.
+
+Hint Extern 1 (_, _ : _ ⊢ _ <: _ : _ | _) => rewrite_for_rename : sized.
+
+Ltac try_sized_constructors :=
+  eapply ss_abs +
+  eapply ss_pi +
+  eapply ss_bind +
+  eapply ss_forall +
+  eapply ss_forall_l +
+  eapply ss_forall_r
+.
+
+Ltac unsized_sized_strategy :=
+  match goal with
+  | _ => solve [eassumption | auto 2 | eauto 2]
+  | _ => progress destruct_exists
+  | |- exists n, _ ⊢ _ <: _ : _ | n => eapply ex_intro
+  | |- _ ⊢ e_bind _ _ <: e_bind _ _ : _ | _ =>
+    let L' := gather_for_weakening in
+    eapply ss_bind with (L := L')
+  | _ => try_sized_constructors
+  | |- ?g =>
+    match g with
+    | context [ [_ / _] _ ] => fail 1
+    | _ => rewrite_for_rename
+    end
+  | _ => solve [eauto 4 using sized_renaming_cons]
+  end
+.
+
+Ltac apply_unsized_sized_strategy :=
+  repeat (intros; unsized_sized_strategy).
+
+Ltac solve_unsized_sized :=
+  try solve
+      [ destruct_exists; eauto 3
+      | (try reconstruct_sub); instantiate_colimits;
+        conclude_freshes; apply_unsized_sized_strategy
+       ].
+
 Lemma unsized_sized : forall Γ e1 e2 A,
     Γ ⊢ e1 <: e2 : A -> exists n, Γ ⊢ e1 <: e2 : A | n.
 Proof.
   intros.
-  induction H; destruct_exists; eauto 3;
-    reconstruct_sub; instantiate_LN_IH_with_fresh.
-  - exists (S (IHusub + IH0 + IH)).
-    solve_unsized_sized_with ss_abs.
-  - exists (S (IHusub1 + IHusub2 + IHusub3 + IH0 + IH)).
-    solve_unsized_sized_with ss_pi.
-  - exists (S (IHusub + IH0 + IH)).
-    solve_unsized_sized_with ss_bind.
-  - exists (S (IHusub1 + IHusub2 + IHusub3 + IH)).
-    solve_unsized_sized_with ss_forall_l.
-  - exists (S (IHusub1 + IHusub2 + IH)).
-    solve_unsized_sized_with ss_forall_r.
-  - exists (S (IHusub + IH)).
-    solve_unsized_sized_with ss_forall.
+  induction H; try solve_unsized_sized.
+  (* a little special for bind, for the strategy inappropriately instantiating freshness
+     involving extracted expression *)
+  - reconstruct_sub.
+    instantiate_colimit H0. instantiate_colimit H1.
+    instantiate_colimit H2. instantiate_colimit H3.
+    conclude_freshes. apply_unsized_sized_strategy.
 Qed.
 
 Fixpoint forall_order (e : expr) : nat :=
@@ -382,8 +417,11 @@ Fixpoint forall_order (e : expr) : nat :=
   | e_pi   A B => forall_order A + forall_order B
   | e_bind A B => forall_order A + forall_order B
   | e_all  A B => S (forall_order A + forall_order B)
+  | e_castup A e => forall_order A + forall_order e
+  | e_castdn A e => forall_order A + forall_order e
   | _ => 0
-  end.
+  end
+.
 
 Fixpoint esize (e : expr) : nat :=
   match e with
@@ -397,7 +435,66 @@ Fixpoint esize (e : expr) : nat :=
   | e_pi   A B => S (esize A + esize B)
   | e_all  A B => S (esize A + esize B)
   | e_bind A B => S (esize A + esize B)
-  end.
+  | e_castup A e => S (esize A + esize e)
+  | e_castdn A e => S (esize A + esize e)
+  end
+.
+
+Lemma open_var_size_eq_rec : forall A x n,
+    esize (A <n> ^^ `x) = esize A.
+Proof.
+  induction A; simpl; intros; auto.
+  now destruct (n0 == n).
+Qed.
+
+Lemma open_var_size_eq : forall A x,
+    esize (A ^` x) = esize A.
+Proof.
+  intros. apply open_var_size_eq_rec.
+Qed.
+
+Lemma open_var_forall_order_eq_rec : forall A x n,
+    forall_order (A <n> ^^ `x) = forall_order A.
+Proof.
+  induction A; simpl; intros; auto.
+  now destruct (n0 == n).
+Qed.
+
+Lemma open_var_forall_order_eq : forall A x,
+    forall_order (A ^` x) = forall_order A.
+Proof.
+  intros. apply open_var_forall_order_eq_rec.
+Qed.
+
+Lemma mono_type_order : forall e,
+    mono_type e -> forall_order e = 0.
+Proof.
+  intros. induction H; simpl; auto;
+  try solve [ now rewrite IHmono_type1, IHmono_type2
+        | instantiate_colimits; rewrite open_var_forall_order_eq in H1;
+          now rewrite IHmono_type, H1].
+Qed.
+
+Lemma open_mono_order_rec : forall e v n,
+    mono_type v -> forall_order (e <n> ^^ v) = forall_order e.
+Proof.
+  induction e; simpl; intros; auto.
+  - destruct (n0 == n).
+    + now apply mono_type_order.
+    + auto.
+Qed.
+
+Lemma open_mono_order : forall e v,
+    mono_type v -> forall_order (e ^^ v) = forall_order e.
+Proof.
+  intros. now apply open_mono_order_rec.
+Qed.
+
+Lemma open_var_order : forall e x,
+    forall_order (e ^` x) = forall_order e.
+Proof.
+  intros. apply open_mono_order. auto.
+Qed.
 
 Ltac extract_eq :=
   match goal with
@@ -410,6 +507,11 @@ Ltac extract_eq :=
     let E := fresh H in
     assert (e = 0) as E by omega;
     clear H; try subst e
+  | H : ?e1 + ?e2 = 0 |- _ =>
+    let E1 := fresh H in
+    let E2 := fresh H in
+    assert (e1 = 0 /\ e2 = 0) as [E1 E2] by omega;
+    clear H; try subst e1 e2
   end
 .
 
@@ -431,26 +533,24 @@ Ltac solve_size_inconsistency :=
   end
 .
 
-
-Ltac find_IHtsz := match goal with
-| H : forall _ _ _ _ _ _ _ _, forall_order _ <= _ -> _ |- _ => H
-end.
-
-Ltac find_IHesz := match goal with
-| H : forall (_ : nat) _ _ _ _ _ _ _ _, forall_order _ <= _ -> _ |- _ => H
-end.
-
-
-Ltac solve_right_subsumption_impl IH := match goal with
-| Hr : ?Γ ⊢ ?e2 <: ?e3 : ?B | ?n2 |- _ ⊢ ?e1 <: ?e3 : ?A => match goal with
-  | _ : Γ ⊢ B <: _ : e_kind ?k | _ |- _ => match goal with
-    | Hl : Γ ⊢ ?e1 <: e2 : A | ?n1 |- _ =>
-       apply IH with e2 B n1 n2; eauto 3; omega
-end end end
+Ltac find_IHorder :=
+  match goal with
+  | H : forall (_ : nat) (_ : nat) _ _ _ _ _ _ _ _,
+      _ + _ + _ <= _ -> _ |- _ => H
+  end
 .
 
-Ltac solve_right_subsumption :=
-  let H := find_IHtsz in solve_right_subsumption_impl H.
+Ltac find_IHesz :=
+  match goal with
+  | H : forall (_ : nat) _ _ _ _ _ _ _ _, _ + _ + _ <= _ -> _ |- _ => H
+  end
+.
+
+Ltac find_IHtsz :=
+  match goal with
+  | H : forall _ _ _ _ _ _ _ _, _ + _ + _ <= _ -> _ |- _ => H
+  end
+.
 
 Ltac solve_left_subsumption_impl IH :=
   match goal with
@@ -464,62 +564,16 @@ end end end
 Ltac solve_left_subsumption :=
   let H := find_IHtsz in solve_left_subsumption_impl H.
 
-Lemma open_var_size_eq_rec : forall A x n,
-    esize (A <^^n> `x) = esize A.
-Proof.
-  induction A; simpl; intros; auto.
-  now destruct (n0 == n).
-Qed.
+Ltac solve_right_subsumption_impl IH := match goal with
+| Hr : ?Γ ⊢ ?e2 <: ?e3 : ?B | ?n2 |- _ ⊢ ?e1 <: ?e3 : ?A => match goal with
+  | _ : Γ ⊢ B <: _ : e_kind ?k | _ |- _ => match goal with
+    | Hl : Γ ⊢ ?e1 <: e2 : A | ?n1 |- _ =>
+       apply IH with e2 B n1 n2; eauto 3; omega
+end end end
+.
 
-Lemma open_var_size_eq : forall A x,
-    esize (A <^> x) = esize A.
-Proof.
-  intros. apply open_var_size_eq_rec.
-Qed.
-
-Lemma open_var_forall_order_eq_rec : forall A x n,
-    forall_order (A <^^n> `x) = forall_order A.
-Proof.
-  induction A; simpl; intros; auto.
-  now destruct (n0 == n).
-Qed.
-
-Lemma open_var_forall_order_eq : forall A x,
-    forall_order (A <^> x) = forall_order A.
-Proof.
-  intros. apply open_var_forall_order_eq_rec.
-Qed.
-
-Lemma mono_type_order : forall e,
-    mono_type e -> forall_order e = 0.
-Proof.
-  intros. induction H; simpl; auto;
-  [> now rewrite IHmono_type1, IHmono_type2
-   | pick fresh x; specialize (H1 x Fr);
-     rewrite open_var_forall_order_eq in H1;
-     now rewrite IHmono_type, H1..].
-Qed.
-
-Lemma open_mono_order_rec : forall e v n,
-    mono_type v -> forall_order (e <^^n> v) = forall_order e.
-Proof.
-  induction e; simpl; intros; auto.
-  - destruct (n0 == n).
-    + now apply mono_type_order.
-    + auto.
-Qed.
-
-Lemma open_mono_order : forall e v,
-    mono_type v -> forall_order (e <^^> v) = forall_order e.
-Proof.
-  intros. now apply open_mono_order_rec.
-Qed.
-
-Lemma open_var_order : forall e x,
-    forall_order (e <^> x) = forall_order e.
-Proof.
-  intros. apply open_mono_order. auto.
-Qed.
+Ltac solve_right_subsumption :=
+  let H := find_IHtsz in solve_right_subsumption_impl H.
 
 Ltac discharge_equality E :=
   try solve [inversion E]; subst; try (rewrite E in *; clear E).
@@ -562,54 +616,36 @@ Ltac star_absurd :=
 Lemma sized_sub_wf : forall Γ e1 e2 A n,
     Γ ⊢ e1 <: e2 : A | n -> ⊢ Γ.
 Proof.
-  intros. apply sized_unsized in H. auto.
+  intros. apply sized_unsized in H.
+  eapply sub_ctx_wf. eassumption.
 Qed.
 
 Hint Resolve sized_weakening_cons : core.
 Hint Resolve sized_sub_wf : core.
 
-Ltac solve_right_forall_r_impl IH :=
-  match goal with
-  | _ : forall x, x `notin` ?L -> ?Γ, x : ?B ⊢ ?e2 <: ?C <^> x : * | ?n2
-        |- ?Γ ⊢ ?e1 <: e_all ?B ?C : * => match goal with
-    | _ : Γ ⊢ e1 <: e2 : * | ?n1 |- _ => match goal with
-      | _ : Γ ⊢ B <: B : e_kind ?k | _ |- _ =>
-        let x := fresh "x" in
-        pick fresh x and apply s_forall_r;
-        [> eauto 3.. |
-         intros; apply IH with (n1 + n2) e2 * n1 n2; eauto 4;
-         try rewrite open_var_size_eq;
-         try rewrite open_var_forall_order_eq; simpl in *; omega]
-      end
-    end
-  end
+Hint Rewrite open_var_size_eq : trans.
+Hint Rewrite open_var_forall_order_eq : trans.
+Hint Rewrite open_mono_order : trans.
 
+Ltac solve_with_IHorder :=
+  instantiate_colimits; match goal with
+  | Hl : _ ⊢ ?e1 <: ?e2 : * | ?n1
+         |- _ ⊢ ?e1 <: ?e3 : * => match goal with
+    | Hr : _ ⊢ e2 <: ?e3 : ?B | ?n2 |- _ =>
+      let IH := find_IHorder in
+      apply IH with (esize e1 + esize e3) (n1 + n2) e2 B n1 n2;
+      eauto 4 using sized_weakening_cons;
+      autorewrite with trans; auto; simpl in *; omega
+     end
+   end
 .
 
 Ltac solve_right_forall_r :=
-  let IH := find_IHesz in solve_right_forall_r_impl IH.
-
-Ltac solve_left_forall_l_impl IH :=
-  match goal with
-  | _ : ?Γ ⊢ ?B0 <^^> ?e <: ?e2 : * | ?n1 |- ?Γ
-        ⊢ e_all ?A ?B0 <: ?e3 : * => match goal with
-    | _ : Γ ⊢ e2 <: e3 : ?B | ?n2 |- _ => match goal with
-      | _ : Γ ⊢ A <: A : e_kind ?k | _ |- _ =>
-        eapply s_forall_l; eauto;
-        apply IH with (esize (B0 <^^> e) + esize e3) (n1 + n2) e2 B n1 n2; eauto;
-        try (rewrite open_mono_order; auto); simpl in *; omega
-      end
-    end
-  end
-.
-
-Ltac find_IHorder1 :=
-  match goal with
-  | H : forall (_ : nat) (_ : nat) _ _ _ _ _ _ _ _, forall_order _ <= _ -> _ |- _ => H
-  end.
+  let x := fresh "x" in
+  pick fresh x and apply s_forall_r for weakening; eauto 3; solve_with_IHorder.
 
 Ltac solve_left_forall_l :=
-  let IH := find_IHorder1 in solve_left_forall_l_impl IH.
+  eapply s_forall_l; eauto 3; solve_with_IHorder.
 
 Theorem substitution_cons : forall Γ x A B e1 e2 e3,
   Γ , x : B ⊢ e1 <: e2 : A ->
@@ -623,7 +659,7 @@ Qed.
 
 Ltac prepare_left_judgement :=
   match goal with
-  | H : forall x, x `notin` ?L -> ?Γ, x : ?B ⊢ ?e1 <: ?C <^> x : * | _
+  | H : forall x, x `notin` ?L -> ?Γ, x : ?B ⊢ ?e1 <: ?C ^` x : * | _
         |- ?Γ ⊢ ?e1 <: ?e3 : * => match goal with
     | _ : mono_type ?e |- _ =>
       let x := fresh "x" in
@@ -631,7 +667,7 @@ Ltac prepare_left_judgement :=
       let Hl := fresh "Hl" in
       let n := fresh "n" in
       pick fresh x for (L `union` fv_expr e1 `union` fv_expr C);
-      assert (H : Γ ⊢ e1 <: C <^^> e : *) by
+      assert (H : Γ ⊢ e1 <: C ^^ e : *) by
         (replace * with ([e / x] * ) by reflexivity;
          rewrite <- (fresh_subst_eq e1 x e); auto;
          rewrite (open_subst_eq C x e); auto;
@@ -641,47 +677,17 @@ Ltac prepare_left_judgement :=
   end
 .
 
-Ltac find_IHorder2 :=
-  match goal with
-  | H : forall (_ : nat) (_ : nat) (_ : nat) _ _ _ _ _ _ _ _,
-      forall_order _ <= _ -> _ |- _ => H
-  end
-.
-
-Ltac specialize_LN_hyps :=
-  repeat match goal with
-  | H : forall x, x `notin` ?L -> _ |- _ , ?x0 : _ ⊢ _ <: _ : _ =>
-    let Fr := fresh "Fr" in
-    assert (Fr : x0 `notin` L) by auto;
-    specialize (H x0 Fr); clear Fr
-  end
-.
-
-
-Ltac solve_with_IHorder2 :=
-  specialize_LN_hyps; match goal with
-  | Hl : ?Γ ⊢ ?e1 <: ?C <^^> ?e : * | ?n1
-         |- ?Γ ⊢ ?e1 <: ?e3 : * => match goal with
-    | Hr : Γ ⊢ C <^^> e <: ?e3 : * | ?n2 |- _ =>
-      let IH := find_IHorder2 in
-      apply IH with (forall_order e1 + forall_order e3)
-                    (esize e1 + esize e3) (n1 + n2) (C <^^> e) * n1 n2; eauto;
-      rewrite open_mono_order; auto; simpl in *; omega
-     end
-   end
-.
-
 Ltac solve_l_forall_r_r_forall :=
-  pick fresh x and apply s_forall_r; eauto;
-  solve_with_IHorder2.
+  pick fresh x and apply s_forall_r; eauto 3;
+  solve_with_IHorder.
 
 
 Ltac solve_l_forall_r_r_forall_l :=
-  prepare_left_judgement; solve_with_IHorder2.
+  prepare_left_judgement; solve_with_IHorder.
 
 Ltac prepare_left_judgement_2 :=
   match goal with
-  | H : forall x, x `notin` ?L -> ?Γ, x : ?A ⊢ ?B <^> x <: ?C <^> x : * | _
+  | H : forall x, x `notin` ?L -> ?Γ, x : ?A ⊢ ?B ^` x <: ?C ^` x : * | _
         |- ?Γ ⊢ e_all ?A ?B <: _ : * => match goal with
     | _ : mono_type ?e |- _ =>
       let x := fresh "x" in
@@ -689,7 +695,7 @@ Ltac prepare_left_judgement_2 :=
       let Hl := fresh "Hl" in
       let n := fresh "n" in
       pick fresh x for (L `union` fv_expr B `union` fv_expr C);
-      assert (H : Γ ⊢ B <^^> e <: C <^^> e : *) by
+      assert (H : Γ ⊢ B ^^ e <: C ^^ e : *) by
         (rewrite (open_subst_eq B x e), (open_subst_eq C x e); auto;
          replace * with ([e / x] * ) by reflexivity;
          eapply substitution_cons; eauto);
@@ -700,26 +706,24 @@ Ltac prepare_left_judgement_2 :=
 
 Ltac solve_l_forall_r_forall_l :=
   prepare_left_judgement_2;
-  pick fresh x and apply s_forall_l; eauto; solve_with_IHorder2.
+  pick fresh x and apply s_forall_l; eauto 4; solve_with_IHorder.
 
 Ltac solve_l_forall_r_forall :=
   match goal with
   | |- _ ⊢ e_all _ _ <: e_all _ _ : _ =>
-    pick fresh x and apply s_forall; eauto; solve_with_IHorder2
+    pick fresh x and apply s_forall; eauto 3; solve_with_IHorder
   end
 .
 
-
 Ltac solve_with_IHtsz :=
-  specialize_LN_hyps;
+  instantiate_colimits;
   match goal with
   | Hl : ?Γ ⊢ ?e1 <: ?e2 : ?A | ?n1 |- ?Γ ⊢ ?e1 <: ?e3 : _ =>
     match goal with
     | Hr : ?Γ ⊢ ?e2 <: ?e3 : ?B | ?n2 |- _ =>
       let IH := find_IHtsz in
-      apply IH with e2 B n1 n2; eauto; simpl in *;
-      try repeat (rewrite open_mono_order; auto);
-      try repeat rewrite open_var_size_eq; omega
+      apply IH with e2 B n1 n2; eauto 3; simpl in *;
+      autorewrite with trans; auto; simpl in *; omega
     end
   end
 .
@@ -734,7 +738,7 @@ Ltac solve_abs :=
 Ltac solve_app :=
   match goal with
   | _ : ?Γ ⊢ ?f1 <: _ : e_pi ?A ?B | _
-      |- ?Γ ⊢ e_app ?f1 _ <: e_app _ _ : ?B <^^> ?e =>
+      |- ?Γ ⊢ e_app ?f1 _ <: e_app _ _ : ?B ^^ ?e =>
     apply s_app with A; eauto; solve_with_IHtsz
   end
 .
@@ -743,6 +747,20 @@ Ltac solve_bind :=
   match goal with
   | |- _ ⊢ e_bind _ _ <: e_bind _ _ : _ =>
     pick fresh x and apply s_bind; eauto; solve_with_IHtsz
+  end
+.
+
+Ltac solve_castup :=
+  match goal with
+  | |- _ ⊢ e_castup _ _ <: e_castup _ _ : _ =>
+    eapply s_castup; try solve_with_IHtsz; eauto
+  end
+.
+
+Ltac solve_castdn :=
+  match goal with
+  | |- _ ⊢ e_castdn _ _ <: e_castdn _ _ : _ =>
+    eapply s_castdn; try solve_with_IHtsz; eauto
   end
 .
 
@@ -758,14 +776,12 @@ Qed.
 
 Ltac solve_with_IHesz :=
   match goal with
-  | _ : ?Γ ⊢ ?e1 <: ?e2 : ?A | ?n1 |- ?Γ ⊢ ?e1 <: ?e3 : ?A =>
+  | _ : ?Γ ⊢ ?e1 <: ?e2 : ?A | ?n1 |- ?Γ ⊢ ?e1 <: ?e3 : _ =>
     match goal with
     | _ : ?Γ ⊢ ?e2 <: ?e3 : ?B | ?n2 |- _ =>
       let IH := find_IHesz in
-      apply IH with (n1 + n2) e2 B n1 n2; eauto;
-      repeat rewrite open_var_size_eq;
-      repeat rewrite open_var_forall_order_eq;
-      simpl in *; omega
+      apply IH with (n1 + n2) e2 B n1 n2; eauto 3;
+      autorewrite with trans; auto; simpl in *; omega
     end
   end
 .
@@ -785,7 +801,7 @@ Ltac narrowing_return_type_ctx :=
 .
 
 Ltac solve_pi_return_type :=
-  specialize_LN_hyps; unify_kinds;
+  instantiate_colimits; unify_kinds;
   narrowing_return_type_ctx; solve_with_IHesz.
 
 Ltac solve_pi :=
@@ -808,11 +824,14 @@ Ltac easy_solves_r :=
       | solve_pi
       | solve_app
       | solve_bind
+      | solve_castdn
+      | solve_castup
       | solve_l_forall_r_r_forall_l
       | solve_l_forall_r_r_forall
       | solve_l_forall_r_forall_l
       | solve_l_forall_r_forall
-      ].
+      ]
+.
 
 Ltac solve_by_case_analysis :=
   match goal with
@@ -825,26 +844,20 @@ Ltac solve_by_case_analysis :=
   end
 .
 
-Theorem transitivity' : forall order2 order1 esz tsz,
+Theorem transitivity' : forall order esz tsz,
     forall Γ e1 e2 e3 A B n1 n2,
-      forall_order e2 <= order2 ->
-      forall_order e1 + forall_order e3 <= order1 ->
+      forall_order e1 + forall_order e2 + forall_order e3 <= order ->
       esize e1 + esize e3 <= esz ->
       n1 + n2 <= tsz ->
       Γ ⊢ e1 <: e2 : A | n1 -> Γ ⊢ e2 <: e3 : B | n2 -> Γ ⊢ e1 <: e3 : A.
 Proof.
-  induction order2; induction order1; induction esz; induction tsz;
-    intros * Eorder2 Eorder1 Eesz Etsz Subl Subr;
+  induction order; induction esz; induction tsz;
+    intros * Eorder Eesz Etsz Subl Subr;
     extract_eqs.
-    all: try solve_tree_size_base.
+  all: try solve_tree_size_base.
   - solve_by_case_analysis.
   - solve_by_case_analysis.
   - solve_by_case_analysis.
-  - solve_by_case_analysis.
-  - solve_by_case_analysis.
-  - solve_by_case_analysis.
-  - solve_by_case_analysis.
-  (* don't worry, the final case takes the longest time :) *)
   - solve_by_case_analysis.
 Qed.
 
@@ -855,6 +868,6 @@ Proof.
   apply unsized_sized in H as (n1 & Hl).
   apply unsized_sized in H0 as (n2 & Hr).
   apply transitivity' with
-      (forall_order e2) (forall_order e1 + forall_order e3)
+      (forall_order e1 + forall_order e2 + forall_order e3)
       (esize e1 + esize e3) (n1 + n2) e2 B n1 n2; eauto.
 Qed.
