Declarative/BasicProperties.v
@@ -3,82 +3,79 @@ Require Import Program.Equality.
 
 Import ListNotations.
 
+Lemma binded_type_correct : forall Γ x A e1 e2 B,
+    Γ, x : A ⊢ e1 <: e2 : B -> exists k, Γ ⊢ A : e_kind k.
+Proof.
+  intros. eauto using wf_ctx_type_correct_cons with wf.
+Qed.
+
+
+Local Ltac conclude_relevant_refl_in_ctx :=
+  repeat match goal with
+  | H : forall x, x `notin` ?L -> ?G, x : ?A ⊢ _ <: _ : _ |- ?g =>
+    match g with
+    | context [A] => progress
+      match goal with
+      | H' : G ⊢ A <: A : _ |- _ => idtac
+      | _ =>
+        let H' := fresh "H" in
+        let k  := fresh "k" in
+        pose colimit H as H';
+        apply binded_type_correct in H' as (k & H')
+      end
+    end
+  end
+.
+
+Theorem reflexivity_l : forall Γ e1 e2 A, Γ ⊢ e1 <: e2 : A -> Γ ⊢ e1 : A.
+Proof.
+  intros. induction H; conclude_relevant_refl_in_ctx; eauto 3.
+Qed.
+
+Theorem reflexivity_r : forall Γ e1 e2 A, Γ ⊢ e1 <: e2 : A -> Γ ⊢ e2 : A.
+Proof.
+  intros. induction H; conclude_relevant_refl_in_ctx; eauto 3.
+Qed.
+
+Ltac gather_for_weakening :=
+  let A := gather_atoms_with (fun x : atoms => x) in
+  let B := gather_atoms_with (fun x : atom => singleton x) in
+  let C := gather_atoms_with (fun x : context => dom x) in
+  constr:(A `union` B `union` C).
+
+Tactic Notation "pick" "fresh" ident(x) "and" "apply" constr(H) "for" "weakening" :=
+  apply_fresh_base_fixed H gather_for_weakening x.
+
+Lemma wf_eauto_helper : forall Γ1 Γ2 x A,
+    ⊢ Γ1 ,, Γ2 , x : A -> ⊢ Γ1 ,, (Γ2 , x : A).
+Proof. easy. Qed.
+
+Hint Resolve wf_eauto_helper : weakening.
+
+Hint Resolve reflexivity_r : refl.
+Hint Resolve reflexivity_l : refl.
+
+Hint Extern 4 (⊢ _ , _ : _) => eauto 4 with refl : weakening.
+
+Ltac something := econstructor 5 with (L := empty).
+
 Theorem weakening : forall Γ1 Γ2 Γ3 e1 e2 A,
     Γ1 ,, Γ3 ⊢ e1 <: e2 : A ->
     ⊢ Γ1 ,, Γ2 ,, Γ3 ->
     Γ1 ,, Γ2 ,, Γ3 ⊢ e1 <: e2 : A.
-Proof.
+Proof with autorewrite with assoc; eauto with weakening.
   intros until A. intro Hsub.
-  dependent induction Hsub; intro Hwf.
-  - apply s_var.
-    + assumption.
-    + now apply var_in_ctx_weakening.
-  - now apply s_lit.
-  - now apply s_star.
-  - now apply s_int.
-  - apply s_abs with (L `union` dom (Γ1 ,, Γ2 ,, Γ3)) k1 k2.
-    + now apply IHHsub.
-    + intros. distribute_ctx. apply H0; simpl; eauto 3.
-    + intros. distribute_ctx. apply H2; simpl; eauto 3.
-  - apply s_pi with (L `union` dom (Γ1 ,, Γ2 ,, Γ3)) k1.
-    + now apply IHHsub1.
-    + now apply IHHsub2.
-    + now apply IHHsub3.
-    + intros. distribute_ctx. apply H0.
-      * auto.
-      * reflexivity.
-      * eapply wf_cons.
-        ** assumption.
-        ** auto.
-        ** now apply IHHsub1.
-    + intros. distribute_ctx. apply H2.
-      * auto.
-      * reflexivity.
-      * eapply wf_cons.
-        ** assumption.
-        ** auto.
-        ** now apply IHHsub2.
-  - apply s_app with A.
-    + assumption.
-    + now apply IHHsub1.
-    + now apply IHHsub2.
-  - apply s_bind with (L `union` dom (Γ1 ,, Γ2 ,, Γ3)) k; auto 2.
-    + intros. distribute_ctx. apply H0; simpl; eauto 4.
-    + intros. distribute_ctx. apply H2; simpl; eauto 4.
-  - apply s_forall_l with (L `union` dom (Γ1 ,, Γ2 ,, Γ3)) e k.
-    + assumption.
-    + now apply IHHsub1.
-    + now apply IHHsub2.
-    + now apply IHHsub3.
-    + intros. distribute_ctx. apply H1.
-      * auto.
-      * reflexivity.
-      * eapply wf_cons.
-        ** assumption.
-        ** auto.
-        ** now apply IHHsub1.
-  - apply s_forall_r with (L `union` dom (Γ1 ,, Γ2 ,, Γ3)) k.
-    + now apply IHHsub1.
-    + now apply IHHsub2.
-    + intros. distribute_ctx. apply H0.
-      * auto.
-      * reflexivity.
-      * eapply wf_cons.
-        ** assumption.
-        ** auto.
-        ** now apply IHHsub1.
-  - apply s_forall with (L `union` dom (Γ1 ,, Γ2 ,, Γ3)) k.
-    + now apply IHHsub.
-    + intros. distribute_ctx. apply H0.
-      * auto.
-      * reflexivity.
-      * eapply wf_cons.
-        ** assumption.
-        ** auto.
-        ** now apply IHHsub.
-  - apply s_sub with A k.
-    + now apply IHHsub1.
-    + now apply IHHsub2.
+  dependent induction Hsub; intro Hwf; auto.
+  - pick fresh x and apply s_abs for weakening...
+  - pick fresh x and apply s_pi for weakening...
+  - apply s_app with A...
+  - pick fresh x and apply s_bind for weakening...
+  - eauto.
+  - eauto.
+  - pick fresh x and apply s_forall_l for weakening...
+  - pick fresh x and apply s_forall_r for weakening...
+  - pick fresh x and apply s_forall for weakening...
+  - eauto.
 Qed.
 
 Corollary weakening_cons : forall Γ x X e1 e2 A,
@@ -86,11 +83,12 @@ Corollary weakening_cons : forall Γ x X e1 e2 A,
     ⊢ Γ , x : X ->
     Γ , x : X ⊢ e1 <: e2 : A.
 Proof.
-  intros.
-  replace (Γ , x : X) with (Γ ,, (x ~ X) ,, nil)  by reflexivity.
+  intros. replace (Γ , x : X) with (Γ ,, (x ~ X) ,, nil) by reflexivity.
   now apply weakening.
 Qed.
 
+Hint Resolve reflexivity_r : core.
+Hint Resolve reflexivity_l : core.
 Hint Resolve weakening_cons : core.
 
 Corollary weakening_app : forall Γ Γ' e1 e2 A,
@@ -98,60 +96,18 @@ Corollary weakening_app : forall Γ Γ' e1 e2 A,
     ⊢ Γ ,, Γ' ->
     Γ ,, Γ' ⊢ e1 <: e2 : A.
 Proof.
-  intros.
-  replace (Γ ,, Γ') with (Γ ,, Γ' ,, nil) by reflexivity.
+  intros. replace (Γ ,, Γ') with (Γ ,, Γ' ,, nil) by reflexivity.
   now apply weakening.
 Qed.
-
-Theorem reflexivity_r : forall Γ e1 e2 A, Γ ⊢ e1 <: e2 : A -> Γ ⊢ e2 : A.
-Proof.
-  intros.
-  induction H.
-  - auto.
-  - auto.
-  - auto.
-  - auto.
-  - apply s_abs with L k1 k2; eauto 3.
-  - apply s_pi with L k1; eauto 3.
-  - apply s_app with A; eauto 3.
-  - apply s_bind with L k; eauto.
-  - assumption.
-  - apply s_forall with L k; eauto.
-  - apply s_forall with L k; eauto.
-  - apply s_sub with A k; eauto.
-Qed.
-
-Theorem reflexivity_l : forall Γ e1 e2 A, Γ ⊢ e1 <: e2 : A -> Γ ⊢ e1 : A.
-Proof.
-  intros. induction H.
-  - now apply s_var.
-  - now apply s_lit.
-  - now apply s_star.
-  - now apply s_int.
-  - eapply s_abs; eauto.
-  - eapply s_pi; eauto.
-  - now apply s_app with A.
-  - now apply s_bind with L k.
-  - apply s_forall with L k.
-    + assumption.
-    + apply H3.
-  - assumption.
-  - apply s_forall with L k; assumption.
-  - eauto.
-Qed.
-
-Hint Resolve reflexivity_r : core.
-Hint Resolve reflexivity_l : core.
 
 Theorem ctx_narrowing : forall Γ1 Γ2 x A B C e1 e2 k,
   Γ1 , x : B ,, Γ2 ⊢ e1 <: e2 : C ->
   Γ1 ⊢ A <: B : e_kind k ->
   Γ1 , x : A ,, Γ2 ⊢ e1 <: e2 : C.
-Proof.
+Proof with autorewrite with assoc; eauto 3.
   intros.
   remember (Γ1 , x : B ,, Γ2) as Γ.
-  generalize HeqΓ. clear HeqΓ.
-  generalize Γ2. clear Γ2.
+  generalize Γ2, HeqΓ. clear HeqΓ Γ2.
   apply sub_mut with
     (P := fun Γ e1 e2 C (_ : Γ ⊢ e1 <: e2 : C) =>
         forall Γ2, Γ = Γ1 , x : B ,, Γ2 -> Γ1 , x : A ,, Γ2 ⊢ e1 <: e2 : C)
@@ -161,21 +117,23 @@ Proof.
     + subst. apply weakening_app; auto.
       assert (A0 = B) by now apply binds_type_equal with Γ1 x0 Γ2. subst.
       apply s_sub with A k.
-      * apply s_var; eauto.
-      * apply weakening_cons; eauto.
+      * apply s_var; eauto with wf.
+      * apply weakening_cons; eauto with wf.
     + apply s_var.
       * auto.
       * now apply binds_type_not_equal with B.
   - auto.
   - auto.
   - auto.
-  - pick fresh x' and apply s_abs; eauto 3.
-  - pick fresh x' and apply s_pi; eauto 3.
+  - pick fresh x' and apply s_abs...
+  - pick fresh x' and apply s_pi...
   - eauto.
-  - pick fresh x' and apply s_bind; eauto 3.
-  - apply s_forall_l with L e k0; eauto 3.
-  - apply s_forall_r with (add x L) k0; auto.
+  - pick fresh x' and apply s_bind...
   - eauto.
+  - eauto.
+  - pick fresh x' and apply s_forall_l...
+  - pick fresh x' and apply s_forall_r...
+  - pick fresh x' and apply s_forall...
   - eauto.
 
   (* ⊢ Γ1 , x : B ,, Γ2 → Γ1 ⊢ A <: B : * → ⊢ Γ1 , x : A ,, Γ2 *)
