Declarative/LanguageUtil.v
@@ -6,13 +6,18 @@ Export ListNotations.
 
 Require Export Metalib.Metatheory.
 
+Scheme sub_mut := Induction for usub       Sort Prop
+  with  wf_mut := Induction for wf_context Sort Prop.
+
 Notation "G ⊢ e : A" := (usub G e e A)
     (at level 65, e at next level, no associativity) : type_scope.
 Notation "G ⊢ e1 <: e2 : A" := (usub G e1 e2 A)
     (at level 65, e1 at next level, e2 at next level, no associativity) : type_scope.
 
-Notation "e1 ⟶ e2"  := (reduce  e1 e2) (at level 60, no associativity) : type_scope.
-Notation "e1 ⋆⟶ e2" := (ereduce e1 e2) (at level 60, no associativity) : type_scope.
+Notation "e1 ⟶ e2"  := (reduce  e1 e2)
+    (at level 60, no associativity) : type_scope.
+Notation "e1 ⋆⟶ e2" := (ereduce e1 e2)
+    (at level 60, no associativity) : type_scope.
 
 Declare Scope ctx_scope.
 Delimit Scope ctx_scope with ctx.
@@ -35,7 +40,7 @@ Notation "` x" := (e_var_f x)
 Notation "G , x : A" := ((x, A) :: G)
     (left associativity, at level 62, x at level 0) : ctx_scope.
 
-Notation "G1 ,, G2" := (G2 ++ G1)
+Notation "G1 ,, G2" := (app G2 G1)
     (left associativity, at level 62) : ctx_scope.
 
 Notation "⊢ G" := (wf_context G)
@@ -47,15 +52,14 @@ Notation "x : A ∈ G" := (binds x A G)
 Notation "x # e" := (x `notin` fv_expr e)
     (no associativity, at level 65) : type_scope.
 
-Notation "e < ^^ n > e' " := (open_expr_wrt_expr_rec n e' e)
+Notation "e < n > ^^ e' " := (open_expr_wrt_expr_rec n e' e)
     (at level 40, n at level 0, left associativity) : expr_scope.
 
-Notation "e <^^> e'" :=
-  (open_expr_wrt_expr e e')
-    (at level 40, no associativity) : expr_scope.
+Notation "e ^^ e'" := (open_expr_wrt_expr e e')
+    (at level 40, left associativity) : expr_scope.
 
-Notation "e <^> x" := (open_expr_wrt_expr e (e_var_f x))
-    (at level 40) : expr_scope.
+Notation "e ^` x" := (open_expr_wrt_expr e (e_var_f x))
+    (at level 40, left associativity) : expr_scope.
 
 Definition subst_ctx (e : expr) (x : exprvar) : context -> context :=
   map (subst_expr e x).
@@ -65,16 +69,21 @@ Notation "[ e1 / x ] e2" := (subst_expr e1 x e2)
 Notation "[ e // x ] ctx" := (subst_ctx e x ctx)
     (at level 60, e at level 0, x at level 0, right associativity) : ctx_scope.
 
+Notation "e ⋆^^ e'" := (open_eexpr_wrt_eexpr e e')
+    (at level 40, left associativity) : eexpr_scope.
 
-Notation "e ⋆^^ e'" := (open_eexpr_wrt_eexpr e e') (at level 40, no associativity) : eexpr_scope.
-Notation "e ⋆^ x" := (open_eexpr_wrt_eexpr e (ee_var_f x)) (at level 40) : eexpr_scope.
+Notation "e ⋆^` x" := (open_eexpr_wrt_eexpr e (ee_var_f x))
+    (at level 40, left associativity) : eexpr_scope.
+
 Notation "[ e1 ⋆/ x ] e2" := (subst_eexpr e1 x e2)
     (at level 60, e1 at level 0, x at level 0, right associativity) : eexpr_scope.
-Notation "e ⋆ n ^^ e'" := (open_eexpr_wrt_eexpr_rec n e' e)
-    (at level 40, n at level 0, no associativity) : eexpr_scope.
 
-Open Scope eexpr_scope.
+Notation "e ⋆ n ^^ e'" := (open_eexpr_wrt_eexpr_rec n e' e)
+    (at level 40, n at level 0, left associativity) : eexpr_scope.
+
 Open Scope ctx_scope.
+Open Scope eexpr_scope.
+Open Scope expr_scope.
 
 Lemma binds__in_dom : forall t Γ x (A : t),
     x : A ∈ Γ -> x `in` dom Γ.
@@ -146,20 +155,22 @@ Proof.
       exists x0. exists (x1 , a : e). reflexivity.
 Qed.
 
+Lemma wf_uncons : forall Γ x A,
+    ⊢ Γ, x : A -> ⊢ Γ.
+Proof.
+  intros. now inversion H.
+Qed.
+
+Hint Resolve wf_uncons : wf.
+
 Theorem sub_ctx_wf : forall Γ e1 e2 A,
   Γ ⊢ e1 <: e2 : A -> ⊢ Γ.
 Proof.
-  intros. induction H; eauto.
+  intros.
+  induction H; solve [assumption | pick fresh x; eauto with wf].
 Qed.
 
-Ltac ctx_wf_auto :=
-  match goal with
-  | _ : ?G ⊢ _ <: _ : _ |- ⊢ ?G =>
-    eapply sub_ctx_wf; eassumption
-  end
-.
-
-Hint Extern 2 (⊢ _) => ctx_wf_auto : core.
+Hint Resolve sub_ctx_wf : wf.
 
 Lemma prefix_wf : forall Γ1 Γ2, ⊢ Γ1 ,, Γ2 -> ⊢ Γ1.
 Proof.
@@ -168,7 +179,7 @@ Proof.
   - inversion H. auto.
 Qed.
 
-Hint Resolve prefix_wf : core.
+Hint Resolve prefix_wf : wf.
 
 Lemma binds_consistent : forall Γ x A B,
     ⊢ Γ -> x : A ∈ Γ -> x : B ∈ Γ -> A = B.
@@ -180,12 +191,20 @@ Qed.
 
 Open Scope expr_scope.
 
-Theorem wf_ctx_type_correct : forall Γ1 Γ2 x A,
+Lemma wf_ctx_type_correct : forall Γ1 Γ2 x A,
   ⊢ Γ1 , x : A ,, Γ2 -> exists k, Γ1 ⊢ A : e_kind k.
 Proof.
   induction Γ2; intros.
   - inversion H. now exists k.
   - inversion H. subst. now apply IHΓ2 with x.
+Qed.
+
+Lemma wf_ctx_type_correct_cons : forall Γ x A,
+    ⊢ Γ, x : A -> exists k, Γ ⊢ A : e_kind k.
+Proof.
+  intros. eapply wf_ctx_type_correct.
+  replace (Γ, x : A) with (Γ, x : A,, nil) in H by reflexivity.
+  eassumption.
 Qed.
 
 Lemma var_in_ctx_weakening : forall Γ2 Γ1 Γ3 x (A : expr),
@@ -199,45 +218,39 @@ Proof.
 Qed.
 
 Theorem fresh_open_rec : forall x e1 e2 n,
-  x # e1 -> x # e2 -> x # open_expr_wrt_expr_rec n e2 e1.
+  x # e1 -> x # e2 -> x # e1 <n> ^^ e2.
 Proof.
   intros x e1.
-  induction e1; simpl; intros e2 n' Hfresh1 Hfresh2; eauto.
+  induction e1; simpl; intros e2 n' Hfresh1 Hfresh2; eauto 4.
   - now destruct (n' == n).
 Qed.
 
 Corollary fresh_open : forall x e1 e2,
-  x # e1 -> x # e2 -> x # open_expr_wrt_expr e1 e2.
+  x # e1 -> x # e2 -> x # e1 ^^ e2.
 Proof.
   intros. now apply fresh_open_rec.
 Qed.
 
 Corollary fresh_open_var : forall x e y,
-  x # e -> x <> y -> x # open_expr_wrt_expr e (e_var_f y).
+  x # e -> x <> y -> x # e ^` y.
 Proof.
-  intros. apply fresh_open.
-  + auto.
-  + simpl. apply notin_singleton_2. intro.
-    symmetry in H1. contradiction.
+  intros. apply fresh_open; auto.
 Qed.
 
 Theorem fresh_close_rec : forall e1 e2 x n,
-    x # open_expr_wrt_expr_rec n e2 e1 -> x # e1.
+    x # e1 <n> ^^ e2 -> x # e1.
 Proof.
-  induction e1; intros; simpl in *; eauto.
+  induction e1; intros; simpl in *; eauto 4.
 Qed.
 
 Theorem fresh_close : forall e1 e2 x,
-    x # e1 <^^> e2 -> x # e1.
+    x # e1 ^^ e2 -> x # e1.
 Proof.
   intros until x. apply fresh_close_rec.
 Qed.
 
-Hint Resolve fresh_open_var : core.
-Hint Resolve fresh_close : core.
-
-Scheme sub_mut := Induction for usub       Sort Prop
-  with  wf_mut := Induction for wf_context Sort Prop.
+Hint Resolve fresh_open_var : fresh.
+Hint Resolve fresh_close : fresh.
 
 Fixpoint context_fresh (x : atom) (ctx : context) : Prop :=
   match ctx with
@@ -248,23 +261,22 @@ Fixpoint context_fresh (x : atom) (ctx : context) : Prop :=
 
 Hint Unfold context_fresh : core.
 
-Ltac distribute_ctx :=
-  match goal with
-  | |- (?g1 ,, ?g2 , ?x : ?A) ⊢ _ <: _ : _ =>
-    replace (g1 ,, g2 , x : A) with
-      (g1 ,, (g2 , x : A)) by auto
-  end
-.
+Lemma ctx_app_cons_assoc : forall (Γ1 Γ2 : context) x A,
+    Γ1 ,, Γ2 , x : A = Γ1 ,, (Γ2 , x : A).
+Proof.
+  easy.
+Qed.
 
-Hint Extern 1 (_ ,, _ , _ : _ ⊢ _ <: _ : _) => distribute_ctx : core.
+Hint Rewrite ctx_app_cons_assoc : assoc.
 
 Lemma open_rec_eq_cancel : forall e e1 e2 m n,
-    m <> n -> e <^^m> e1 <^^n> e2 = e <^^m> e1 ->
-    e <^^n> e2 = e.
+    m <> n -> e <m> ^^ e1 <n> ^^ e2 = e <m> ^^ e1 ->
+    e <n> ^^ e2 = e.
 Proof.
-  induction e; simpl; intros; auto;
+  induction e; simpl; intros; auto 3;
     try solve
-      [inversion H0; apply IHe1 in H2; auto; apply IHe2 in H3; auto; congruence].
+        [inversion H0 as [[Hinv1 Hinv2]];
+         (apply IHe1 in Hinv1; apply IHe2 in Hinv2); (auto || congruence)].
   - destruct (m == n).
     + destruct (n0 == n); congruence.
     + simpl in H0. destruct (n0 == n); easy.
@@ -273,18 +285,19 @@ Qed.
 Hint Resolve open_rec_eq_cancel : ln.
 
 Lemma lc_open_eq : forall e,
-    lc_expr e -> forall n e', e <^^n> e' = e.
+    lc_expr e -> forall n e', e <n> ^^ e' = e.
 Proof.
-  intros e LC. induction LC; simpl; intros; auto;
+  intros e LC. induction LC; simpl; intros;
     try solve
-        [ pick fresh x; rewrite IHLC;
-          erewrite open_rec_eq_cancel with (m := 0); eauto].
-  - now (rewrite IHLC1; rewrite IHLC2).
+        [ reflexivity
+        | pick fresh x; rewrite IHLC;
+          erewrite open_rec_eq_cancel with (m := 0); eauto
+        | now (rewrite IHLC1; rewrite IHLC2)].
 Qed.
 
 Lemma subst_open_rec_distr : forall e x v e' n,
     lc_expr v ->
-    [v / x] e <^^n> e' = ([v / x] e) <^^n> ([v / x] e').
+    [v / x] e <n> ^^ e' = ([v / x] e) <n> ^^ ([v / x] e').
 Proof.
   induction e; simpl; intros; auto;
     try solve [rewrite IHe1; auto; rewrite IHe2; auto].
@@ -294,21 +307,23 @@ Qed.
 
 Lemma subst_open_distr : forall e x v e',
     lc_expr v ->
-    [v / x] e <^^> e' = ([v / x] e) <^^> ([v / x] e').
+    [v / x] e ^^ e' = ([v / x] e) ^^ ([v / x] e').
 Proof.
   intros. unfold open_expr_wrt_expr. now rewrite subst_open_rec_distr.
 Qed.
 
 Lemma subst_open_var_assoc : forall e x v y,
     y <> x -> lc_expr v ->
-    ([v / x] e) <^> y = [v / x] e <^> y.
+    ([v / x] e) ^` y = [v / x] e ^` y.
 Proof.
   intros.
-  assert ([v / x] e <^> y = ([v / x] e) <^^> ([v / x] `y))
+  assert ([v / x] e ^` y = ([v / x] e) ^^ ([v / x] `y))
     by now apply subst_open_distr.
   assert ([v / x] `y = `y) by (simpl; destruct (y == x); easy).
   now rewrite H2 in H1.
 Qed.
+
+Hint Rewrite subst_open_var_assoc : assoc.
 
 Lemma fresh_subst_eq : forall e x e', x # e -> [e' / x] e = e.
 Proof.
@@ -321,7 +336,7 @@ Qed.
 
 Lemma open_subst_eq : forall e x v,
     x # e -> lc_expr v ->
-    e <^^> v = [v / x] e <^> x.
+    e ^^ v = [v / x] e ^` x.
 Proof.
   intros.
   rewrite subst_open_distr. simpl.
@@ -338,8 +353,7 @@ Proof.
   - destruct (x0 == x); auto.
 
   Ltac solve_inductive_case_with C :=
-    let L := gather_atoms in
-    apply C with L; auto; intros; rewrite subst_open_var_assoc; auto.
+    pick fresh x' and apply C; auto; intros; rewrite subst_open_var_assoc; auto.
 
   - solve_inductive_case_with lc_e_abs.
   - solve_inductive_case_with lc_e_pi.
@@ -348,8 +362,8 @@ Proof.
 Qed.
 
 Lemma lc_open_preserve : forall e e',
-    (exists L, forall x, x `notin` L -> lc_expr (e <^> x)) ->
-    lc_expr e' -> lc_expr (e <^^> e').
+    (exists L, forall x, x `notin` L -> lc_expr (e ^` x)) ->
+    lc_expr e' -> lc_expr (e ^^ e').
 Proof.
   intros e e' [L H] H'.
   pick fresh x for (fv_expr e `union` L).
@@ -357,7 +371,6 @@ Proof.
   rewrite (open_subst_eq _ _ _ H0 H').
   apply lc_subst; auto.
 Qed.
-
 
 Fixpoint lc_ctx (c : context) : Prop :=
   match c with
@@ -368,32 +381,81 @@ Fixpoint lc_ctx (c : context) : Prop :=
 
 Import Program.Tactics.
 
-Ltac destruct_all_with x :=
-  match goal with
-  | H : forall x', x' `notin` ?L -> ?A /\ ?B |- _ =>
-    let H1 := fresh in
-    let H2 := fresh in
-    destruct H with x' as [H1 H2]; try assumption; clear H; destruct_all_with x
-  | _ => destruct_pairs
+Ltac instantiate_colimit_with H x :=
+  match type of H with
+  | forall x, x `notin` ?L -> _ =>
+    let H1 := fresh "H" in
+    assert (H1 : x `notin` L) by eauto;
+    specialize (H x H1); clear H1
+  | ?e => idtac e
   end
 .
 
+Ltac instantiate_colimits_with x :=
+  repeat match goal with
+  | H : forall x, x `notin` ?L -> _ |- _ =>
+    instantiate_colimit_with H x
+  end
+.
+
+Ltac detect_fresh_var_and_do t :=
+  match goal with
+  | Fr : ?x `notin` ?L1 |- _ => t x
+  | _ =>
+    let x := fresh "x" in
+    pick fresh x; t x
+  end
+.
+
+Ltac instantiate_colimits :=
+  detect_fresh_var_and_do instantiate_colimits_with.
+
+Ltac instantiate_colimit H :=
+  let f x := instantiate_colimit_with H x in
+  detect_fresh_var_and_do f
+.
+
+Ltac pose_colimit_with H x H' :=
+  match type of H with
+  | forall x, x `notin` ?L -> _ =>
+    let Fr := fresh "Fr" in
+    assert (Fr : x `notin` L) by eauto;
+    pose proof (H x Fr) as H'; clear Fr
+  end
+.
+
+Ltac pose_colimit H H' :=
+  let f x := pose_colimit_with H x H' in
+  detect_fresh_var_and_do f
+.
+
+Tactic Notation "pose" "colimit" ident(H) :=
+  let H' := fresh H in
+  pose_colimit H H'.
+
+Tactic Notation "pose" "colimit" ident(H) "as" ident(H') :=
+  pose_colimit H H'.
+
 Lemma usub_lc : forall Γ e1 e2 A,
-    Γ ⊢ e1 <: e2 : A -> lc_expr e1 /\ lc_expr e2 /\ lc_expr A.
+    Γ ⊢ e1 <: e2 : A -> lc_ctx Γ /\ lc_expr e1 /\ lc_expr e2 /\ lc_expr A.
 Proof.
-  intros.
+  Local Ltac solve_with_pairs_in_colimits := instantiate_colimits; destruct_pairs; auto.
+
   apply sub_mut with
       (P := fun c e1 e2 A (_ : c ⊢ e1 <: e2 : A) =>
-        lc_expr e1 /\ lc_expr e2 /\ lc_expr A)
-      (P0 := fun c (_ : ⊢ c) => lc_ctx c) (c := Γ); simpl; intros;
-    destruct_pairs; repeat split; auto;
-      try solve [econstructor; auto; intros; destruct_all_with x; auto].
+        lc_ctx c /\ lc_expr e1 /\ lc_expr e2 /\ lc_expr A)
+      (P0 := fun c (_ : ⊢ c) => lc_ctx c); simpl; intros; auto;
+    try solve
+        [repeat split;
+         solve [ solve_with_pairs_in_colimits
+               | econstructor; intros; solve_with_pairs_in_colimits]].
+
   - induction G. inversion b.
-    destruct a. destruct H0. inversion w. subst. destruct b.
-    + inversion H2. now subst.
-    + now apply IHG.
-  - inversion H3; subst.
-    apply lc_open_preserve; eauto.
+    destruct a, H. inversion w. subst. destruct b.
+    + inversion H1. now subst.
+    + simpl. destruct IHG as (lc_G & lc_x & lc_x' & lc_A); auto.
+  - repeat split; destruct_pairs; auto.
+    inversion H3. subst. eauto using lc_open_preserve.
 Qed.
 
 Lemma mono_lc : forall e,
@@ -407,9 +469,12 @@ Ltac solve_basic_lc :=
   | H : _ ⊢ ?e <: _ : _ |- lc_expr ?e => apply usub_lc in H
   | H : _ ⊢ _ <: ?e : _ |- lc_expr ?e => apply usub_lc in H
   | H : _ ⊢ _ <: _ : ?e |- lc_expr ?e => apply usub_lc in H
-  | H : mono_type ?e |- lc_expr ?e => now apply mono_lc
+  | H : forall x, x `notin` ?L -> _, x : ?A ⊢ _ <: _ : _ |- lc_expr ?A =>
+    instantiate_colimit H; apply usub_lc in H; simpl in H
   end; destruct_pairs; assumption
 .
+
+Hint Resolve mono_lc : core.
 
 Hint Extern 1 (lc_expr _) => solve_basic_lc : core.
 
@@ -455,39 +520,18 @@ Proof.
   induction H; simpl; auto.
   (* var *)
   - destruct (x0 == x); auto.
-  - apply mono_pi with (add x L).
+  - pick fresh x' and apply mono_pi.
     + assumption.
-    + intros. rewrite subst_open_var_assoc.
-      apply H2. all: auto.
-  - apply mono_lambda with (add x L).
+    + autorewrite with assoc; auto.
+  - pick fresh x' and apply mono_lambda.
     + assumption.
-    + intros. rewrite subst_open_var_assoc.
-      apply H2. all: auto.
-  - apply mono_bind with (add x L).
+    + autorewrite with assoc; auto.
+  - pick fresh x' and apply mono_bind.
     + assumption.
-    + intros. rewrite subst_open_var_assoc.
-      apply H2. all: auto.
+    + autorewrite with assoc; auto.
 Qed.
 
-Ltac instantiate_colimit x H :=
-  match type of H with
-  | forall x, x `notin` ?L -> _ =>
-    let H1 := fresh "H" in
-    assert (H1 : x `notin` L) by eauto;
-    specialize (H x H1); clear H1
-  end
-.
-
-
-Ltac instantiate_colimits :=
-  match goal with
-  | Fr : ?x `notin` ?L1 |- _ => repeat
-    match goal with
-    | H : forall x, x `notin` ?L2 -> _ |- _ =>
-      instantiate_colimit x H
-    end
-  end
-.
+Hint Resolve subst_mono : core.
 
 Ltac instantiate_trivial_equals := repeat
   match goal with
@@ -496,4 +540,71 @@ Ltac instantiate_trivial_equals := repeat
   end
 .
 
-Hint Extern 1 (lc_expr _) => instantiate_colimits : inst.
+Lemma strengthen_colimit : forall L' P L ,
+    (forall x, x `notin` L -> P x) ->
+    (forall x, x `notin` (L `union` L') -> P x).
+Proof.
+  intros. auto.
+Qed.
+
+(*
+Adjusting the colimit requirement in the hypothesis to
+help 'eauto' inferring the often-omitted cofinite lists
+*)
+Ltac adjust_colimits L' :=
+  repeat
+    match goal with
+    | H : forall x, x `notin` ?L -> _ |- _ =>
+      match L with
+      | context [L'] => fail 1
+      | _ =>
+        let H' := fresh H in
+        pose proof (strengthen_colimit L' _ _ H) as H';
+        simpl in H'; clear H
+      end
+    end
+.
+
+Ltac adjust_colimits_for gather :=
+  let L := gather in
+  adjust_colimits L.
+
+(*
+1. Using the '+' tactical to enable backtracking in case of fail on
+   branches of one constructor
+2. Putting s_forall in front of s_forall_l and s_forall_r,
+   and omitting s_sub to prevent potential infinite loop, when
+   try_constructors are put into a repeat match loop
+*)
+Ltac try_constructors :=
+  eapply s_abs +
+  eapply s_pi +
+  eapply s_app +
+  eapply s_bind +
+  eapply s_castup +
+  eapply s_castdn +
+  eapply s_forall +
+  eapply s_forall_l +
+  eapply s_forall_r.
+
+(*
+Neither gather_atoms_with in Metalib, or gather_vars_with in TLC
+allows `F` to be a tactic function.
+*)
+Ltac gather_atoms_with_tactic F :=
+  let rec gather V :=
+    match goal with
+    | H: ?S |- _ =>
+      let FH := F H in
+      match V with
+      | context [FH] => fail 1
+      | _ => gather (FH `union` V)
+      end
+    | _ => V
+    end in
+  let L := gather empty in eval simpl in L.
+
+Ltac apply_fresh_base_fixed H gather_vars atom_name :=
+  let L := gather_vars in
+  let L := beautify_fset L in
+  pick fresh atom_name excluding L and apply H.
