Declarative/Properties.v
@@ -23,20 +23,55 @@ Qed.
 
 Lemma subst_ctx_distr_cons : forall Γ x A y e,
     [e // y] Γ , x : [e / y] A = [e // y] (Γ , x : A).
-Proof.
-  intros. reflexivity.
-Qed.
+Proof. reflexivity. Qed.
 
 Lemma ctx_app_cons_assoc : forall (Γ1 Γ2 : context) x A,
     Γ1 ,, Γ2 , x : A = Γ1 ,, (Γ2 , x : A).
+Proof. reflexivity. Qed.
+
+Hint Rewrite ctx_app_cons_assoc : substitution.
+Hint Rewrite subst_ctx_distr_cons : substitution.
+Hint Rewrite subst_open_var_assoc : substitution.
+Hint Rewrite subst_extract : substitution.
+
+Ltac crush_lc :=
+  repeat
+    match goal with
+    | |- forall x, x `notin` _ -> lc_expr _ => intros
+    | _ => first
+            [ progress auto
+            | progress eauto using lc_subst, lc_open_preserve
+            | progress autorewrite with assoc; auto ]
+    | H : ?T |- lc_expr (?e ^^ _) =>
+      match T with
+      | context [lc_expr ?T2] =>
+        match T2 with
+        | context [e] => inversion H; subst
+        end
+      end
+    | |- lc_expr ([_ / _] _) => apply lc_subst
+    end
+.
+
+Hint Extern 1 (lc_expr _) => crush_lc : lc.
+Hint Extern 1 (forall x, x `notin` _ -> lc_expr _) => crush_lc : lc.
+
+Lemma value_subst : forall e x v,
+    lc_expr v -> value e -> value ([v / x] e).
 Proof.
-  reflexivity.
+  intros * Lc V. induction V; simpl; eauto with lc.
 Qed.
 
-Hint Rewrite ctx_app_cons_assoc : reassoc.
-Hint Rewrite subst_ctx_distr_cons : reassoc.
-Hint Rewrite subst_open_var_assoc : reassoc.
-Hint Rewrite subst_extract : reassoc.
+Hint Resolve mono_lc : mono.
+Hint Resolve subst_mono : mono.
+Hint Resolve value_subst : value.
+
+Lemma reduce_subst : forall A B,
+    A ⟶ B -> forall x e, mono_type e -> ([e / x] A) ⟶ ([e / x] B).
+Proof with try rewrite subst_open_distr; eauto with lc mono value.
+  intros A B Hr.
+  induction Hr; simpl; intros...
+Qed.
 
 Lemma dom_subst_equal : forall Γ x v,
     dom ([v // x] Γ) = dom Γ.
@@ -46,12 +81,41 @@ Proof.
   + destruct a. simpl. now rewrite (IHΓ x v).
 Qed.
 
-Local Ltac solve_substitution :=
-  try solve
-      [ auto
-      | intros; autorewrite with reassoc;
-        (auto 2 || eauto using fv_subst_inclusion)
-      ].
+Ltac subst_gather_helper e :=
+  match type of e with
+  | mono_type ?t => constr:(fv_eexpr (extract t))
+  end
+.
+
+Ltac gather_for_substitution :=
+  let L1 := gather_atoms_with (fun L : atoms => L) in
+  let L2 := gather_atoms_with (fun x : atom => singleton x) in
+  let L3 := gather_atoms_with_tactic subst_gather_helper in
+  constr:(L1 `union` L2 `union` L3).
+
+Ltac substitution_strategy :=
+  match goal with
+  | _ => solve [auto 3]
+  | _ => progress autorewrite with substitution
+  | |- _ ⊢ e_app _ _ <: e_app _ _ : [_ / _] _ ^^ _ =>
+    (* [v / x] A ^^ e = [v / x] A ^^ [v / x] e *)
+    rewrite -> subst_open_distr
+  | |- _ ⊢ ([?v / ?x] ?e1) ^^ _ <: _ : _ =>
+    rewrite <- subst_open_distr
+  | |- _ `notin` fv_eexpr _ => solve [eauto 4 using fv_subst_inclusion]
+  | |- _ ⟶ _ => solve [eauto using reduce_subst]
+  | _ => try_constructors
+  | _ => solve [eauto]
+  end
+.
+
+Ltac apply_substitution_strategy :=
+  repeat (intros; substitution_strategy).
+
+Ltac solve_subst :=
+  solve [
+      adjust_colimits_for gather_for_substitution;
+      apply_substitution_strategy].
 
 Theorem substitution : forall Γ1 Γ2 x A B e1 e2 e3,
   Γ1 , x : B ,, Γ2 ⊢ e1 <: e2 : A ->
@@ -74,24 +138,21 @@ Proof.
       rewrite fresh_subst_eq. apply weakening_app; auto.
       apply prefix_wf in w. inversion w. subst.
       eapply fresh_ctx_fresh_expr; eauto.
-    + apply s_var. auto.
-      apply binds_subst with B; auto.
-  - auto.
-  - auto.
-  - auto.
-  - pick fresh x' and apply s_abs; solve_substitution.
-  - pick fresh x' and apply s_pi ; solve_substitution.
-  - rewrite subst_open_distr; auto.
-    apply s_app with ([e3 / x] A0); auto using subst_mono.
-  - apply s_bind with (add x L `union` fv_eexpr (extract e3)) k;
-      solve_substitution.
+    + apply s_var. auto. apply binds_subst with B; auto.
+  - solve_subst.
+  - solve_subst.
+  - solve_subst.
+  - solve_subst.
+  - solve_subst.
+  - solve_subst.
+  - solve_subst.
+  - solve_subst.
+  - solve_subst.
   - apply s_forall_l with (add x L) ([e3 / x] e) k;
-      solve_substitution.
-    + now apply subst_mono; auto.
-    + rewrite <- subst_open_distr; auto.
-  - pick fresh x' and apply s_forall_r; solve_substitution.
-  - pick fresh x' and apply s_forall; solve_substitution.
-  - eauto.
+      apply_substitution_strategy.
+  - solve_subst.
+  - solve_subst.
+  - solve_subst.
 
   - destruct Γ2; inversion H.
   - destruct Γ2; inversion H1; subst; simpl in *.
@@ -131,18 +192,18 @@ Theorem type_correctness : forall Γ e1 e2 A,
     Γ ⊢ e1 <: e2 : A -> A = BOX \/ exists k, Γ ⊢ A : e_kind k.
 Proof.
   intros * Sub.
-  induction Sub; eauto 4.
+  induction Sub; eauto with wf.
   - eauto 3 using ctx_type_correct.
   - pick fresh x.
     destruct (H2 x Fr) as [H' | [k H']].
     + auto.
-    + apply kind_sub_inversion_l in H' as (E1 & E2 & E3). subst. eauto.
+    + apply kind_sub_inversion_l in H' as (E1 & E2 & E3). subst. eauto with wf.
   - destruct IHSub2 as [H0 | [k H0]]. inversion H0.
     dependent induction H0.
-    + clear IHusub1 IHusub2 IHusub3 H0 H2.
+    + clear H1 H3 IHusub IHusub.
       pick fresh x for (L `union` fv_expr B).
       assert (Fr2 : x `notin` L) by auto.
-      specialize (H1 x Fr2).
+      specialize (H2 x Fr2).
       right. exists k.
       rewrite open_subst_eq with (x := x); auto.
       replace (e_kind k) with ([e / x] e_kind k) by reflexivity.
